src/compiler/core/Floor1_haskabelle.thy
@@ -1,0 +1,73 @@
+(******************************************************************************
+ * Haskabelle --- Converting Haskell Source Files to Isabelle/HOL Theories.
+ *                http://isabelle.in.tum.de/repos/haskabelle
+ *
+ * Copyright (c) 2007-2015 Technische Universität München, Germany
+ *               2017-2018 Virginia Tech, USA
+ *
+ * All rights reserved.
+ *
+ * Redistribution and use in source and binary forms, with or without
+ * modification, are permitted provided that the following conditions are
+ * met:
+ *
+ *     * Redistributions of source code must retain the above copyright
+ *       notice, this list of conditions and the following disclaimer.
+ *
+ *     * Redistributions in binary form must reproduce the above
+ *       copyright notice, this list of conditions and the following
+ *       disclaimer in the documentation and/or other materials provided
+ *       with the distribution.
+ *
+ *     * Neither the name of the copyright holders nor the names of its
+ *       contributors may be used to endorse or promote products derived
+ *       from this software without specific prior written permission.
+ *
+ * THIS SOFTWARE IS PROVIDED BY THE COPYRIGHT HOLDERS AND CONTRIBUTORS
+ * "AS IS" AND ANY EXPRESS OR IMPLIED WARRANTIES, INCLUDING, BUT NOT
+ * LIMITED TO, THE IMPLIED WARRANTIES OF MERCHANTABILITY AND FITNESS FOR
+ * A PARTICULAR PURPOSE ARE DISCLAIMED. IN NO EVENT SHALL THE COPYRIGHT
+ * OWNER OR CONTRIBUTORS BE LIABLE FOR ANY DIRECT, INDIRECT, INCIDENTAL,
+ * SPECIAL, EXEMPLARY, OR CONSEQUENTIAL DAMAGES (INCLUDING, BUT NOT
+ * LIMITED TO, PROCUREMENT OF SUBSTITUTE GOODS OR SERVICES; LOSS OF USE,
+ * DATA, OR PROFITS; OR BUSINESS INTERRUPTION) HOWEVER CAUSED AND ON ANY
+ * THEORY OF LIABILITY, WHETHER IN CONTRACT, STRICT LIABILITY, OR TORT
+ * (INCLUDING NEGLIGENCE OR OTHERWISE) ARISING IN ANY WAY OUT OF THE USE
+ * OF THIS SOFTWARE, EVEN IF ADVISED OF THE POSSIBILITY OF SUCH DAMAGE.
+ ******************************************************************************)
+
+section\<open>Main Translation for: Haskabelle\<close>
+
+theory  Floor1_haskabelle
+imports Core_init
+begin
+
+definition "hsk_name = (\<lambda> l_name.
+ \<lambda> Name n \<Rightarrow> n
+ | QName (ThyName n0) n1 \<Rightarrow> 
+    (case List.find (\<lambda>(n1, _). n0 \<triangleq> n1) l_name of
+       None \<Rightarrow> S.flatten [n0, \<open>.\<close>, n1]
+     | Some (_, Some n0) \<Rightarrow> S.flatten [n0, \<open>.\<close>, n1]
+     | Some (_, None) \<Rightarrow> n1))"
+
+definition "hsk_name' names = mk_quote o hsk_name names"
+
+fun hsk_type where
+   "hsk_type names e =
+ (\<lambda> Type n [] \<Rightarrow> Typ_base (hsk_name names n)
+  | Type n l \<Rightarrow> Typ_apply (Typ_base (hsk_name names n)) (map (hsk_type names) l)
+  | Func t1 t2 \<Rightarrow> Typ_apply (hsk_type names t1) [hsk_type names t2]
+  | TVar n \<Rightarrow> Typ_base (hsk_name' names n)) e"
+
+definition "hsk_typespec names = (\<lambda> TypeSpec l n \<Rightarrow> (hsk_name names n, L.map (hsk_name' names) l))"
+
+definition "hsk_stmt old_datatype names =
+  List.map_filter
+   (\<lambda> Meta_HKB.Datatype l \<Rightarrow>
+        Some (O.datatype (Datatype old_datatype (L.map (map_prod (hsk_typespec names) (L.map (map_prod (hsk_name names) (L.map (hsk_type names))))) l)))
+    | TypeSynonym [(t0, t1)] \<Rightarrow> Some (O.type_synonym (Type_synonym (hsk_typespec names t0) (hsk_type names t1)))
+    | Function (Function_Stmt Primrec l1 l2) \<Rightarrow> None)"
+
+definition "print_haskell = (\<lambda> IsaUnit old_datatype l_name name_new [Module (ThyName name_old) _ m _] \<Rightarrow> Pair (hsk_stmt old_datatype ((name_old, Some name_new) # l_name) m))"
+
+end
